theories/contexts.v
@@ -1,0 +1,276 @@
+(** Properties of Wasm label/evaluation contexts *)
+
+From mathcomp Require Import ssreflect ssrfun ssrnat ssrbool eqtype seq.
+From Coq Require Import Program.Equality NArith ZArith.
+From Wasm Require Export common operations datatypes_properties properties.
+
+Set Implicit Arguments.
+Unset Strict Implicit.
+Unset Printing Implicit Defensive.
+
+Ltac decide_eq_arg x y :=
+  let Heq := fresh "Heq" in
+  let Hcontra := fresh "Hcontra" in
+  destruct (x == y) eqn:Heq; move/eqP in Heq; subst; last by right; move => Hcontra; injection Hcontra.
+
+(* Decidable equality of lholed *)
+Definition lholed_eq_dec : forall k (lh1 lh2 : lholed k), {lh1 = lh2} + {lh1 <> lh2}.
+Proof.
+  elim.
+  {
+    move => lh1 lh2.
+    (* TODO: avoid using dependent destruction to remove dependency on axioms like eq_rect_eq *)
+    dependent destruction lh1.
+    dependent destruction lh2.
+    decide_eq_arg l l1.
+    decide_eq_arg l0 l2.
+    by left.
+  }
+  {
+    move => n IH lh1 lh2.
+    dependent destruction lh1.
+    dependent destruction lh2.
+    decide_eq_arg l l2.
+    decide_eq_arg n0 n1.
+    decide_eq_arg l0 l3.
+    decide_eq_arg l1 l4.
+    destruct (IH lh1 lh2) as [ | Hneq]; subst; first by left.
+    right. move => Hcontra; apply Hneq.
+    clear - Hcontra.
+    inversion Hcontra.
+    (* This one should be axiom free -- check *)
+    apply Eqdep_dec.inj_pair2_eq_dec in H0 => //.
+    decide equality.
+  }
+Defined.
+
+Definition lholed_eqb {k} (v1 v2: lholed k) : bool := lholed_eq_dec v1 v2.
+
+Definition eqlholedP {k} :=
+  eq_dec_Equality_axiom (@lholed_eq_dec k).
+
+Canonical Structure lholed_eqMixin {k} := EqMixin (@eqlholedP k).
+Canonical Structure lholed_eqType {k} := Eval hnf in EqType (@lholed k) (@lholed_eqMixin k).
+
+
+Lemma lfilled_not_nil {k}: forall (lh: lholed k) es es', lfill lh es = es' -> es <> [::] -> es' <> [::].
+Proof.
+  elim => /=.
+  { move => vs ? es ? <- ?.
+    by destruct es, vs => //.
+  }
+  { move => k' vs n es lh' IH vs' ?? <- ?.
+    by destruct vs.
+  }
+Qed.
+
+
+(** label context arithmetics **)
+Fixpoint empty_vs_base {k} (lh: lholed k) : bool :=
+  match lh with
+  | LH_base [::] _ => true
+  | LH_rec _ _ _ _ lh _ => empty_vs_base lh
+  | _ => false
+  end.
+
+Fixpoint lh_push_base_vs {k} (lh: lholed k) rvs: lholed k :=
+  match lh with
+  | LH_base vs es => LH_base (vs ++ rvs) es
+  | LH_rec _ vs n es lh' es' =>
+      let lh_pushed := lh_push_base_vs lh' rvs in
+      LH_rec vs n es lh_pushed es'
+  end.
+
+Definition lh_push_front_vs {k} vcs (lh: lholed k): lholed k :=
+  match lh with
+  | LH_base vs es => LH_base (vcs ++ vs) es
+  | LH_rec _ vs n es lh' es' => LH_rec (vcs ++ vs) n es lh' es'
+  end.
+
+Definition lh_drop_vs {k} l (lh: lholed k): lholed k :=
+  match lh with
+  | LH_base vs es => LH_base (drop l vs) es
+  | LH_rec _ vs n es lh' es' => LH_rec (drop l vs) n es lh' es'
+  end.
+
+Definition lh_drop_vs_o {k} l (lh: lholed k): option (lholed k) :=
+  match lh with
+  | LH_base vs es =>
+      if l <= length vs then Some (LH_base (drop l vs) es)
+      else None
+  | LH_rec _ vs n es lh' es' =>
+      if l <= length vs then Some (LH_rec (drop l vs) n es lh' es')
+      else None
+  end.
+
+Definition lh_push_back_es {k} es0 (lh: lholed k): lholed k :=
+  match lh with
+  | LH_base vs es => LH_base vs (es ++ es0)
+  | LH_rec _ vs n es lh' es' => LH_rec vs n es lh' (es' ++ es0)
+  end.
+
+Lemma lfill_push_base_vs {k} : forall (lh: lholed k) vs ves es,
+  ves = v_to_e_list vs ->
+  lfill lh (ves ++ es) = lfill (lh_push_base_vs lh vs) es.
+Proof.
+  induction lh as [vs es | ? vs n es lh' IH es'']; intros rvs vcs e ->; simpl in *.
+  - by rewrite/v_to_e_list map_cat -catA -catA.
+  - do 3 f_equal.
+    by eapply IH; eauto.
+Qed.
+
+Lemma lfill_push_base_vs' {k}: forall (lh: lholed k) vs ves es l,
+    ves = v_to_e_list vs ->
+    length ves >= l ->
+    lfill lh (ves ++ es) = lfill (lh_push_base_vs lh (take (length ves - l) vs)) ((drop (length ves - l) ves) ++ es).
+Proof.
+  move => lh vs ves es l Hves Hlen.
+  rewrite -(cat_take_drop (length ves - l) ves) -catA.
+  erewrite <-lfill_push_base_vs; eauto.
+  subst.
+  repeat rewrite catA cat_take_drop v_to_e_take.
+  by rewrite length_is_size v_to_e_size catA cat_take_drop.
+Qed.
+
+Lemma lfill_push_front_vs {k} : forall (lh: lholed k) vs es LI,
+    lfill lh es = LI ->
+    lfill (lh_push_front_vs vs lh) es = v_to_e_list vs ++ LI.
+Proof.
+  move => lh vs es LI <-.
+  by destruct lh => //=; rewrite - v_to_e_cat -catA.
+Qed.
+
+Lemma lfill_drop_impl {k}: forall (lh: lholed k) ves e es LI,
+    const_list ves ->
+    is_const e = false ->
+    lfill lh (e :: es) = ves ++ LI ->
+    lh_drop_vs_o (length ves) lh = Some (lh_drop_vs (length ves) lh).
+Proof.
+  move => lh ves e es LI Hconst Hnconst Heq.
+  destruct lh; simpl in * => //.
+  all: apply es_split_by_non_const in Heq; eauto; (try by apply v_to_e_const); destruct Heq as [? Heq].
+  all: replace (length ves <= length l) with true; (apply f_equal with (f := @size administrative_instruction) in Heq; rewrite size_cat v_to_e_size in Heq; simpl in Heq; repeat rewrite length_is_size; by lias).
+Qed.
+  
+Lemma lfill_drop_vs {k}: forall (lh: lholed k) ves e es LI,
+    const_list ves ->
+    is_const e = false ->
+    lfill lh (e :: es) = ves ++ LI ->
+    lfill (lh_drop_vs (length ves) lh) (e :: es) = LI.
+Proof.
+  move => lh ves e es LI Hconst Hnconst Heq.
+  destruct lh; simpl in * => //.
+  all: specialize (es_split_by_non_const Heq) as Heq2; destruct Heq2 as [xs Heq2]; eauto; (try by apply v_to_e_const).
+  all: rewrite -(cat_take_drop (length ves) l) -v_to_e_cat -catA in Heq.
+  all: apply concat_cancel_first_n in Heq; last by rewrite v_to_e_size size_take; apply f_equal with (f := size) in Heq2; rewrite v_to_e_size size_cat in Heq2; rewrite length_is_size; destruct (size ves < size l) eqn:?; lias.
+  all: move/andP in Heq; destruct Heq as [Heqves HeqLI]; move/eqP in Heqves; by move/eqP in HeqLI.
+Qed.
+
+Lemma lfill_push_back_es {k}: forall (lh: lholed k) es es0,
+    lfill (lh_push_back_es es0 lh) es = lfill lh es ++ es0.
+Proof.
+  move => lh es es0.
+  destruct lh; simpl in * => //; by repeat rewrite -catA => //.
+Qed.
+
+
+Fixpoint ai_gen_measure (e: administrative_instruction) : nat :=
+  match e with
+  | AI_label _ _ es => 1 + List.list_max (map ai_gen_measure es)
+  | _ => 0
+  end.
+
+Definition ais_gen_measure (LI: list administrative_instruction) : nat :=
+  List.list_max (map ai_gen_measure LI).
+
+Definition lholed_cast {k k'} (lh: lholed k) (Heq: k = k'): lholed k' :=
+  eq_rect k lholed lh k' Heq.
+
+Lemma lfill_const: forall k (lh: lholed k) e lf,
+    const_list lf ->
+    lfill lh [::e] = lf ->
+    {vs & {es & {Heq: k = 0 & lholed_cast lh Heq = (LH_base vs es) /\ lf = v_to_e_list vs ++ [::e] ++ es}}}.
+Proof.
+  move => k lh.
+  destruct lh as [lvs les | k lvs j lces lh les] => //.
+  - move => e lf /=Hconst Hlf.
+    subst.
+    apply const_list_split in Hconst as [_ Hconst].
+    simpl in Hconst.
+    move/andP in Hconst; destruct Hconst as [? Hconst].
+    destruct e as [b | | | |] => //; destruct b => //.
+    exists lvs, les, (Logic.eq_refl 0).
+    by split => //.
+  - move => e lf Hconst Hlf. subst.
+    exfalso.
+    apply const_list_split in Hconst as [_ Hconst].
+    by simpl in Hconst.
+Qed.
+
+Lemma const_seq_factorise (fe: nat -> administrative_instruction) (ves: list administrative_instruction):
+  {vs & {es & ves = v_to_e_list vs ++ [::fe 0] ++ es}} + {forall vs es, ves <> v_to_e_list vs ++ [::fe 0] ++ es}.
+Proof.
+  move: fe.
+  induction ves as [ | e ves']; move => fe; first by right; destruct vs => //.
+  destruct (e == fe 0) eqn:H; move/eqP in H.
+  - subst.
+    left; by exists nil, ves'.
+  - destruct (is_const e) eqn:Hconst.
+    { destruct e as [ b | | | |] => //; destruct b => //.
+      destruct (IHves' fe) as [[vs [es ->]] | Hcontra]; first by left; exists (v :: vs), es.
+      right; move => vs es Heq.
+      destruct vs as [| v0 vs'] => //; simpl in *; first by inversion Heq.
+      apply (Hcontra vs' es) => /=; by inversion Heq.
+    }
+    { right; move => vs es Heq.
+      destruct vs as [| v0 vs'] => //; simpl in *; by inversion Heq; subst.
+    }
+Qed.
+    
+Definition lf_decide fe es: Type := {n & {lh: lholed n | lfill lh [::fe n] = es}} + {forall n (lh: lholed n), lfill lh [::fe n] <> es}.
+
+Definition lfill_factorise_aux (fe: nat -> administrative_instruction) (es: list administrative_instruction) (Hrec: forall fe es', (ais_gen_measure es' < ais_gen_measure es)%coq_nat -> lf_decide fe es'):
+    lf_decide fe es.
+Proof.
+  (* First, decide if lfill0 hold *)
+  destruct (const_seq_factorise fe es) as [[vs' [es'' Heq]] | Hcontra]; first by left; exists 0, (LH_base vs' es'').
+  (* If not, then look at the top of instruction stack *)
+  destruct (split_vals_e es) as [vs es'] eqn:Hsplit.
+  destruct es' as [| e es'].
+  (* Instruction stack is empty *)
+  - right. move => n lh Hlf.
+    apply split_vals_inv in Hsplit as ->; rewrite cats0 in Hlf.
+    rewrite cats0 in Hcontra.
+    apply lfill_const in Hlf; last by apply v_to_e_const.
+    destruct Hlf as [vs' [es [-> [? Heq]]]]; simpl in *; subst.
+    by apply Hcontra in Heq.
+  - specialize (split_vals_nconst Hsplit) as Hnconst.
+    apply split_vals_inv in Hsplit as ->.
+    destruct e as [ | | | j lvs les |].
+    4: {
+      destruct (Hrec (fun n => fe (S n)) les) as [IH | IH] => /=.
+      (* measure *)
+      {
+        unfold ais_gen_measure.
+        rewrite - cat1s map_cat map_cat cat_app cat_app.
+        repeat rewrite List.list_max_app => /=.
+        destruct (List.list_max (map ai_gen_measure es')); by lias.
+      }
+      { destruct IH as [n' [lh' Hlf]].
+        left.
+        exists (S n'), (LH_rec vs j lvs lh' es') => /=.
+        by rewrite Hlf.
+      }
+      { right. move => n lh Hlf.
+        destruct lh as [lvs' les' | n' lvs' les' lh' les'']; simpl in *; first by apply (Hcontra lvs' les').
+        apply const_list_concat_inv in Hlf as [Heq [Heqlab <-]] => //; try by apply v_to_e_const.
+        apply v_to_e_inj in Heq as ->.
+        injection Heqlab as <- <- <-.
+        by eapply IH.
+      }
+    }
+    all: right; move => n' lh Hlf; destruct lh as [lvs' les' | n' lvs' les' lh' les'']; simpl in *; (try by apply (Hcontra lvs' les')); apply const_list_concat_inv in Hlf as [Heq [Heqlab <-]] => //; by apply v_to_e_const.
+Defined.
+
+Program Fixpoint lfill_factorise fe es {measure (ais_gen_measure es)} :=
+  @lfill_factorise_aux fe es lfill_factorise.
