theories/opsem_properties.v
@@ -1,0 +1,36 @@
+From Wasm Require Export opsem properties contexts.
+From mathcomp Require Import ssreflect ssrfun ssrnat ssrbool eqtype seq.
+From Coq Require Import Program NArith ZArith Wf_nat.
+
+Set Implicit Arguments.
+Unset Strict Implicit.
+Unset Printing Implicit Defensive.
+
+Section Host.
+
+Variable host_function: eqType.
+Variable host_instance: host host_function.
+
+Local Definition reduce := @reduce host_function host_instance.
+
+Lemma reduce_not_nil : forall hs hs' σ1 f es σ2 f' es',
+  reduce hs σ1 f es hs' σ2 f' es' -> es <> [::].
+Proof.
+  move => hs hs' σ1 f es σ2 f' es' Hred.
+  elim: {σ1 f es f' σ2} Hred => //;
+    try solve [ repeat intro;
+                match goal with
+                | H : (_ ++ _)%SEQ = [::] |- _ =>
+                  by move: (app_eq_nil _ _ H) => [? ?]
+                end ].
+  { move => e e' _ _ _ Hreds He.
+    rewrite He in Hreds.
+    apply: not_reduce_simple_nil.
+    apply: Hreds. }
+  { intros. destruct ves => //. }
+  { intros. destruct ves => //. }
+  { intros. by destruct ves => //. }
+  { intros. apply: lfilled_not_nil. exact H1. exact H0. }
+Qed.
+
+End Host.
