theories/tactic.v
@@ -102,6 +102,10 @@ Ltac invert_e_typing:=
 
 Ltac auto_basic :=
   repeat lazymatch goal with
+  | |- context C [v_to_e _] =>
+    unfold v_to_e    
+  | |- context C [vs_to_es _] =>
+    unfold vs_to_es
   | |- es_is_basic [::AI_basic _; AI_basic _; AI_basic _; AI_basic _] =>
     simpl; repeat split
   | |- es_is_basic [::AI_basic _; AI_basic _; AI_basic _] =>
